Simplified and improved ghost state type.

veric/own.v
@@ -11,39 +11,27 @@ Local Open Scope pred.
 
 Notation ghost_approx m := (ghost_fmap (approx (level m)) (approx (level m))).
 
-(* Ghost state construction drawn from "Iris from the ground up", Jung et al. *)
-Program Definition ghost_is {I} {RAs: I -> Ghost} g pds dom: pred rmap :=
-  fun m => exists Hv, ghost_of m = ghost_approx m (GHOST _ _ g pds Hv dom).
+(* Ownership construction based on "Iris from the ground up", Jung et al. *)
+Program Definition ghost_is g: pred rmap :=
+  fun m => ghost_of m = ghost_approx m g.
 Next Obligation.
-  intros ???????? (? & Hg).
+  intros ???? Hg.
   rewrite (age1_ghost_of _ _ H), Hg.
   pose proof (age_level _ _ H).
   rewrite ghost_fmap_fmap, approx_oo_approx', approx'_oo_approx by omega; eauto.
 Qed.
 
-Definition Own {I} {RAs: I -> Ghost} g pds dom: pred rmap := allp noat && ghost_is g pds dom.
+Definition Own g: pred rmap := allp noat && ghost_is g.
 
-Lemma Own_valid: forall {I} {RAs: I -> Ghost} g pds dom,
-  Own g pds dom |-- !!ghost.valid g.
-Proof.
-  intros.
-  intros ??.
-  destruct H as (? & ? & ?); auto.
-Qed.
-
-Lemma Own_op: forall {I} {RAs: I -> Ghost} a b c pdsa pdsb pdsc doma domb domc,
-  join a b c -> join pdsa pdsb pdsc ->
-  Own c pdsc domc = Own a pdsa doma * Own b pdsb domb.
+Lemma Own_op: forall a b c, join a b c -> Own c = Own a * Own b.
 Proof.
   intros; apply pred_ext.
-  - intros w (Hno & ? & Hg).
-    assert (ghost.valid a) as Hva by (eapply join_valid; eauto).
-    assert (ghost.valid b) as Hvb by (eapply join_valid; eauto).
-    destruct (make_rmap (resource_at w) (ghost_approx w (GHOST _ _ _ _ Hva doma)) (rmap_valid w) (level w))
+  - intros w (Hno & Hg).
+    destruct (make_rmap (resource_at w) (ghost_approx w a) (rmap_valid w) (level w))
       as (wa & Hla & Hra & Hga).
     { extensionality; apply resource_at_approx. }
     { rewrite ghost_fmap_fmap, approx_oo_approx; auto. }
-    destruct (make_rmap (resource_at w) (ghost_approx w (GHOST _ _ _ _ Hvb domb)) (rmap_valid w) (level w))
+    destruct (make_rmap (resource_at w) (ghost_approx w b) (rmap_valid w) (level w))
       as (wb & Hlb & Hrb & Hgb).
     { extensionality; apply resource_at_approx. }
     { rewrite ghost_fmap_fmap, approx_oo_approx; auto. }
@@ -52,34 +40,17 @@ Proof.
       * intro; rewrite Hra, Hrb.
         apply identity_unit', Hno.
       * rewrite Hg, Hga, Hgb.
-        apply ghost_fmap_join; constructor; auto.
+        apply ghost_fmap_join; auto.
     + simpl; rewrite Hla, Hlb, Hra, Hrb, Hga, Hgb; simpl; eauto 6.
-  - intros w (w1 & w2 & J & (Hnoa & ? & Hga) & (Hnob & ? & Hgb)).
+  - intros w (w1 & w2 & J & (Hnoa & Hga) & (Hnob & Hgb)).
     split.
     + intro l; apply (resource_at_join _ _ _ l) in J.
       simpl in *; rewrite <- (Hnoa _ _ _ J); auto.
     + destruct (join_level _ _ _ J) as [Hl1 Hl2].
       apply ghost_of_join in J.
-      rewrite Hga, Hgb in J; inv J; repeat inj_pair_tac.
-      assert (c1 = c) by (eapply join_eq; eauto); subst.
-      simpl; rewrite <- H9.
-      eexists; apply ghost_ext; auto.
+      rewrite Hga, Hgb in J.
       eapply join_eq; eauto.
-      rewrite Hl1, Hl2.
-      intros i n; specialize (H0 i n); inv H0; constructor.
-      inv H6; auto.
-  Unshelve.
-  apply Hvc.
-Qed.
-
-Lemma preds_join_i: forall {I} a b, (forall i n x y, a i n = Some x -> b i n = Some y -> x = y) ->
-  preds_join I a b (fun i n => match a i n with Some x => Some x | _ => b i n end).
-Proof.
-  intros.
-  intros i n; specialize (H i n).
-  destruct (a i n); [|constructor].
-  destruct (b i n); constructor.
-  specialize (H _ _ eq_refl eq_refl); subst; auto.
+      rewrite Hl1, Hl2; apply ghost_fmap_join; auto.
 Qed.
 
 Lemma ghost_joins_approx: forall n a c,
@@ -88,49 +59,62 @@ Lemma ghost_joins_approx: forall n a c,
     forall b, joins b (ghost_fmap (approx (S n)) (approx (S n)) c') ->
       joins (ghost_fmap (approx n) (approx n) b) (ghost_fmap (approx n) (approx n) c).
 Proof.
-  intros.
-  destruct a as [?? ga pdsa], c as [?? gc pdsc], H as [? H]; inv H; repeat inj_pair_tac.
-  assert (forall i n pp, match pdsa i n, pdsc i n with Some x, Some _ => Some x | _, _ => pdsc i n end = Some pp ->
-    exists a, finmap_get (gc i) n = Some a) as dom'.
-  { intros; destruct (pdsa i n0) eqn: Hi; eauto.
-    destruct (pdsc i n0) eqn: Hi'; inv H; eauto. }
-  eexists (GHOST _ _ gc _ Hv0 dom'); split.
-  - eexists; constructor; eauto.
-    apply preds_join_i; intros.
-    destruct (pdsa i n0); inv H.
-    destruct (pdsc i n0); inv H0; auto.
-  - intros [?? gb pdsb] [? J]; inv J; repeat inj_pair_tac.
-    eexists; constructor; eauto.
-    apply preds_join_i; intros.
-    specialize (H10 i n0); specialize (H11 i n0); simpl in *.
-    destruct (pdsb i n0); inv H.
-    destruct (pdsc i n0); inv H0.
-    destruct (pdsa i n0); inv H10; inv H11.
-    + inv H2; inv H4.
-      rewrite <- H, preds_fmap_fmap, approx_oo_approx', approx'_oo_approx; auto.
-    + inv H3.
-      rewrite preds_fmap_fmap, approx_oo_approx', approx'_oo_approx; auto.
+  intros ???; revert a; induction c; intros.
+  - exists nil; split.
+    + eexists; constructor.
+    + eexists; constructor.
+  - destruct H; inv H.
+    + destruct a0; inv H1.
+      exists (a :: c); split.
+      { eexists; constructor. }
+      intros ? []; eexists.
+      apply ghost_fmap_join with (f := approx n)(g := approx n) in H.
+      rewrite ghost_fmap_fmap, approx_oo_approx', approx'_oo_approx in H by auto; eauto.
+    + destruct a0; inv H0.
+      destruct (IHc a0) as (c' & ? & Hc'); eauto.
+      inv H3.
+      * destruct o; inv H1.
+        exists (a :: c'); split.
+        { destruct H; eexists; constructor; eauto; constructor. }
+        intros ? [? J]; inv J; [eexists; constructor|].
+        destruct (Hc' m1); eauto.
+        eexists; constructor; eauto.
+        instantiate (1 := option_map (fun '(a, b) => (a, preds_fmap (approx n) (approx n) b)) a3).
+        inv H3.
+        -- destruct a as [[]|]; [simpl | constructor].
+           rewrite preds_fmap_fmap, approx_oo_approx', approx'_oo_approx by auto; constructor; auto.
+        -- destruct a; inv H4; constructor.
+        -- destruct a as [[]|]; inv H1; constructor.
+           destruct a2, a5; inv H4; constructor; auto; simpl in *.
+           inv H2.
+           rewrite preds_fmap_fmap, approx_oo_approx', approx'_oo_approx by auto; constructor; auto.
+      * destruct a; inv H2.
+        exists (None :: c'); split.
+        { destruct H; eexists; constructor; eauto; constructor. }
+        intros ? [? J]; inv J; [eexists; constructor|].
+        destruct (Hc' m1); eauto.
+        eexists; constructor; eauto; constructor.
+      * destruct o as [[]|], a as [[]|]; inv H0; inv H1.
+        eexists (Some (s0, _) :: c'); split.
+        { destruct H.
+          destruct a4; inv H2; simpl in *.
+          inv H.
+          eexists (Some (_, _) :: _); constructor; eauto; constructor.
+          constructor; [constructor; eauto | simpl; constructor; eauto]. }
+        intros ? [? J]; inv J; [eexists; constructor|].
+        destruct (Hc' m1); eauto.
+        eexists; constructor; eauto.
+        instantiate (1 := option_map (fun '(a, b) => (a, preds_fmap (approx n) (approx n) b)) a3).
+        inv H4.
+        -- destruct a4; inv H2; simpl in *.
+           inv H3.
+           rewrite <- H2, preds_fmap_fmap, approx_oo_approx', approx'_oo_approx by auto; constructor.
+        -- constructor.
+           destruct a2, a4, a6; inv H2; inv H6; constructor; auto; simpl in *.
+           inv H3; inv H4.
+           rewrite <- H6, preds_fmap_fmap, approx_oo_approx', approx'_oo_approx by auto; constructor; auto.
   Unshelve.
-  apply Hvc.
-  simpl; intros.
-  specialize (H9 i); apply finmap_get_join with (i0 := n0) in H9.
-  destruct (finmap_get (c0 i) n0); eauto.
-  destruct (pdsa i n0) eqn: Hi; inv H.
-  destruct (dom _ _ _ Hi) as [? Hget]; rewrite Hget in H9.
-  destruct (finmap_get (gc i) n0); inv H9.
-  destruct (pdsc i n0) eqn: Hi'; inv H1.
-  destruct (dom0 _ _ _ Hi') as [? Hget]; rewrite Hget in H9.
-  destruct (finmap_get (ga i) n0); inv H9.
-  apply Hvc0.
-  simpl; intros.
-  specialize (H8 i); apply finmap_get_join with (i0 := n0) in H8.
-  destruct (finmap_get (c1 i) n0); eauto.
-  destruct (pdsb i n0) eqn: Hi; inv H.
-  destruct (dom1 _ _ _ Hi) as [? Hget]; rewrite Hget in H8.
-  destruct (finmap_get (gc i) n0); inv H8.
-  destruct (pdsc i n0) eqn: Hi'; inv H1.
-  destruct (dom0 _ _ _ Hi') as [? Hget]; rewrite Hget in H8.
-  destruct (finmap_get (gb i) n0); inv H8.
+  auto.
 Qed.
 
 Program Definition bupd (P: pred rmap): pred rmap :=
@@ -217,16 +201,13 @@ Definition ghost_fp_update_ND a B :=
   forall n c, joins (ghost_fmap (approx n) (approx n) a) c ->
     exists b, B b /\ joins (ghost_fmap (approx n) (approx n) b) c.
 
-Lemma Own_update_ND: forall {I} {RAs: I -> Ghost} a pds Hv dom B,
-  ghost_fp_update_ND (GHOST _ _ a pds Hv dom) B ->
-  Own a pds dom |-- bupd (EX b : _, EX pdsb : _, EX Hvb : _, EX domb : _,
-    !!(B (GHOST _ _ b pdsb Hvb domb)) && Own b pdsb domb).
+Lemma Own_update_ND: forall a B, ghost_fp_update_ND a B ->
+  Own a |-- bupd (EX b : _, !!(B b) && Own b).
 Proof.
   repeat intro.
-  destruct H0 as (Hno & Hv' & Hg).
+  destruct H0 as (Hno & Hg).
   rewrite Hg in H1.
   destruct H1 as [? J].
-  replace Hv' with Hv in J by apply proof_irr.
   destruct (H (level a0) (ghost_approx a0 c)) as (g' & ? & J').
   { eexists; eauto. }
   exists (ghost_fmap (approx (level a0)) (approx (level a0)) g'); split; auto.
@@ -236,10 +217,7 @@ Proof.
   { extensionality; apply resource_at_approx. }
   { rewrite ghost_fmap_fmap, approx_oo_approx; auto. }
   exists m'; repeat split; auto.
-  destruct g' as [?? b pdsb Hvb domb].
-  destruct c; inv J; repeat inj_pair_tac.
-  destruct J' as [? J']; inv J'; repeat inj_pair_tac; subst.
-  exists b, pdsb, Hvb, domb; repeat split; auto.
+  exists g'; repeat split; auto.
   - simpl in *; intro; rewrite Hr; auto.
   - simpl; rewrite Hg', Hl; simpl; eauto.
 Qed.
@@ -267,204 +245,80 @@ Proof.
       [rewrite approx_oo_approx' | rewrite approx'_oo_approx]; auto; omega. }
 Qed.
 
-Lemma Own_update: forall {I} {RAs: I -> Ghost} a pds Hv dom b pdsb Hvb domb,
-  ghost_fp_update (GHOST _ _ a pds Hv dom) (GHOST _ _ b pdsb Hvb domb) ->
-  Own a pds dom |-- bupd (Own b pdsb domb).
+Lemma Own_update: forall a b, ghost_fp_update a b ->
+  Own a |-- bupd (Own b).
 Proof.
   intros; eapply derives_trans.
-  - eapply (Own_update_ND _ _ _ _ (Ensembles.Singleton _ _)).
+  - eapply (Own_update_ND _ (Ensembles.Singleton _ _)).
     repeat intro.
     eexists; split; [constructor|].
     apply H; eauto.
   - apply bupd_mono.
     repeat (apply exp_left; intro).
-    apply prop_andp_left; intro X; inv X; repeat inj_pair_tac.
-    replace x2 with domb by apply proof_irr; auto.
+    apply prop_andp_left; intro X; inv X; auto.
 Qed.
 
-Lemma Own_unit: emp |-- EX a : _, !!(identity a) && match a with GHOST _ _ a pds _ dom =>
-  Own a pds dom end.
+Lemma Own_unit: emp |-- EX a : _, !!(identity a) && Own a.
 Proof.
   intros w ?; simpl in *.
-  exists (ghost_of w); destruct (ghost_of w) eqn: Hw; split; [|split].
-  - rewrite <- Hw; apply ghost_of_identity; auto.
+  exists (ghost_of w); split; [|split].
+  - apply ghost_of_identity; auto.
   - intro; apply resource_at_identity; auto.
-  - eexists; rewrite <- Hw.
-    rewrite ghost_of_approx; auto.
+  - rewrite ghost_of_approx; auto.
 Qed.
 
-Definition gname := {I : Type & I * nat}%type.
+Definition singleton {A} k (x : A) : list (option A) := repeat None k ++ Some x :: nil.
 
-Definition singleton {A} k (x : A) : finmap A := repeat None k ++ Some x :: nil.
-
-Lemma singleton_get: forall {A} k (x : A) j,
-  finmap_get (singleton k x) j = if eq_dec j k then Some x else None.
-Proof.
-  intros; unfold finmap_get, singleton.
-  destruct (eq_dec j k).
-  - subst; rewrite app_nth2; rewrite repeat_length; [|omega].
-    rewrite minus_diag; auto.
-  - destruct (lt_dec j k).
-    + rewrite app_nth1 by (rewrite repeat_length; auto).
-      apply nth_repeat.
-    + rewrite app_nth2; rewrite repeat_length; [|omega].
-      destruct (j - k)%nat eqn: Hd; [omega|].
-      simpl; apply nth_nil.
-Qed.
-
-Program Definition single_ghost {I} {_ : EqDec I} {RAs} {RA} n {H: RAs (fst n) = RA} (a: @G RA) :
-  @G Global_Ghost := fun j => if eq_dec j (fst n) then singleton (snd n) _ else nil.
-Next Obligation.
-Proof.
-  intros; subst; auto.
-Defined.
-
-Definition single_pred {I} {_ : EqDec I} (n: I * nat) (pp: preds) :=
-  fun j m => if eq_dec j (fst n) then if eq_dec m (snd n) then Some pp else None else None.
-
-Lemma single_dom {I} {_ : EqDec I} {RAs} {RA} n (H: RAs (fst n) = RA) (a: @G RA) pp :
-  forall i m p, single_pred n pp i m = Some p ->
-  exists x, finmap_get (single_ghost(H := H) n a i) m = Some x.
-Proof.
-  unfold single_pred, single_ghost; intros.
-  destruct (eq_dec _ _); [|discriminate].
-  rewrite singleton_get.
-  if_tac; inv H0; eauto.
-Qed.
+Definition gname := nat.
 
 Definition own {RA: Ghost} (n: gname) (a: G) (pp: preds) :=
-  match n with existT A n =>
-    EX _ : EqDec A, EX RAs : _, EX H : RAs (fst n) = RA, Own _ _ (single_dom n H a pp) end.
+  EX v : _, Own (singleton n (existT _ RA (exist _ a v), pp)).
 
-(* Because the type of the ghost state is existentially quantified in the rmap, inG has to be a
-   state predicate instead of a pure assertion. *)
-Program Definition inG (RA: Ghost): pred rmap :=
-  (fun m => match ghost_of m with GHOST A RAs g _ _ _ =>
-    exists A_eq : EqDec A, exists inG : {i | RAs i = RA}, True end) && emp.
-Next Obligation.
-  repeat intro.
-  subst filtered_var program_branch_0; simpl in *.
-  rewrite (age1_ghost_of _ _ H).
-  destruct (ghost_of a) eqn: Ha; auto.
+Definition list_set {A} (m : list (option A)) k v : list (option A) :=
+  firstn k m ++ repeat None (k - length m) ++ Some v :: skipn (S k) m.
+
+Lemma singleton_join_gen: forall k a c (m: ghost)
+  (Hjoin: join (Some a) (nth k m None) (Some c)),
+  join (singleton k a) m (list_set m k c).
+Proof.
+  induction k; intros.
+  - destruct m; simpl in *; subst; inv Hjoin; constructor; constructor; auto.
+  - destruct m; simpl in *.
+    + inv Hjoin; constructor.
+    + constructor; [constructor | apply IHk; auto].
 Qed.
 
-Lemma inG_emp: forall RA, inG RA |-- emp.
+Lemma map_repeat : forall {A B} (f : A -> B) x n, map f (repeat x n) = repeat (f x) n.
 Proof.
-  intro; apply andp_left2; auto.
+  induction n; auto; simpl.
+  rewrite IHn; auto.
 Qed.
 
-Lemma andp_emp_derives_dup : forall P, P && emp |-- P && emp * (P && emp).
+Lemma ghost_fmap_singleton: forall f g k v, ghost_fmap f g (singleton k v) =
+  singleton k (match v with (a, b) => (a, preds_fmap f g b) end).
 Proof.
-  intros ???.
-  exists a; exists a; split; auto.
-  apply sepalg.identity_unit'; destruct H; auto.
+  intros; unfold ghost_fmap, singleton.
+  rewrite map_app, map_repeat; auto.
 Qed.
 
-Corollary andp_emp_dup : forall P, P && emp = (P && emp) * (P && emp).
+Lemma ghost_alloc: forall {RA: Ghost} a pp, ghost.valid a ->
+  emp |-- bupd (EX g: gname, own g a pp).
 Proof.
-  intro; apply pred_ext.
-  - apply andp_emp_derives_dup.
-  - apply andp_right.
-    + eapply derives_trans; [apply sepcon_derives, andp_left2, derives_refl; apply andp_left1, derives_refl |].
-      rewrite sepcon_emp; auto.
-    + eapply derives_trans; [apply sepcon_derives; apply andp_left2, derives_refl |].
-      rewrite sepcon_emp; auto.
-Qed.
-
-Lemma inG_dup: forall RA, inG RA |-- inG RA * inG RA.
-Proof.
-  intro; setoid_rewrite <- andp_emp_dup; auto.
-Qed.
-
-Lemma skipn_all: forall {A} (n : nat) (l : list A), (length l <= n)%nat -> skipn n l = nil.
-Proof.
-  induction n; destruct l; auto; simpl; intros; try omega.
-  apply IHn; omega.
-Qed.
-
-Opaque skipn.
-
-Lemma join_fresh: forall {A} {J: Join A} (m : finmap A) v,
-  join (singleton (fresh m) v) m (finmap_set m (fresh m) v).
-Proof.
-  intros; unfold singleton, finmap_set, fresh; simpl.
-  rewrite firstn_all, minus_diag, skipn_all by omega; simpl.
-  induction m; simpl; constructor; auto.
-  constructor.
-Qed.
-
-
-Lemma single_valid: forall {I} {I_eq : EqDec I} {RAs: I -> Ghost} {RA} n (H: RAs (fst n) = RA)
-  (a: @G RA), ghost.valid a -> ghost.valid (single_ghost(H := H) n a).
-Proof.
-  unfold single_ghost; repeat intro.
-  destruct (eq_dec i (fst n)); [|rewrite finmap_get_empty in H1; discriminate].
-  rewrite singleton_get in H1.
-  destruct (eq_dec i0 (snd n)); inv H1; auto.
-Qed.
-
-Lemma ghost_alloc: forall {RA: Ghost} a pp,
-  ghost.valid a ->
-  inG RA |-- bupd (EX g: gname, own g a pp).
-Proof.
-  repeat intro; simpl in *.
-  destruct H1; inv H1.
-  rewrite <- H2 in H0.
-  destruct H0 as [(? & [i e] & _) Hemp].
-  eexists (ghost_approx (level a0) (GHOST _ RA0 (fun j => match eq_dec j i with
-    | left H => singleton (fresh (b j)) ((fun _ _ => _) e H) | _ => nil end)
-    (fun j n => if eq_dec j i then if eq_dec n (fresh (b j)) then Some pp
-                 else None else None) _ _)).
-  set (g' := ghost_approx _ _).
-  split.
-  - eexists; constructor.
-    + instantiate (1 := fun j => if eq_dec j i then _ else _).
-      hnf; intro j.
-      destruct (eq_dec _ _); [|constructor].
-      apply join_fresh.
-    + instantiate (1 := fun j n => if eq_dec j i then if eq_dec n (fresh (b j)) then _ else _ else _).
-      intros j n.
-      destruct (eq_dec _ _); [|constructor].
-      destruct (eq_dec _ _); [|constructor].
-      assert (pdsb j n = None) as ->; [|constructor].
-      destruct (pdsb j n) eqn: Hj; auto.
-      destruct (domb _ _ _ Hj) as [? Hget]; subst j n.
-      rewrite fresh_spec in Hget; discriminate.
-  - destruct (make_rmap (resource_at a0) g' (rmap_valid a0) (level a0)) as (m' & Hl & Hr & Hg).
-    { extensionality; apply resource_at_approx. }
-    { subst g'; rewrite ghost_fmap_fmap, !approx_oo_approx; auto. }
-    exists m'; repeat split; auto.
-    exists (existT _ A (i, fresh (b i))).
-    exists _, _, e; split; simpl.
-    + intro; rewrite Hr; apply resource_at_identity; auto.
-    + rewrite Hl, Hg; subst g'.
-      eexists; apply ghost_ext.
-      * extensionality j.
-        unfold single_ghost; simpl.
-        destruct (eq_dec _ _); auto.
-        rewrite e0; auto.
-      * extensionality j n.
-        unfold single_pred; simpl.
-        destruct (eq_dec _ _); subst; auto.
-  Unshelve.
-  { repeat intro.
-    destruct (eq_dec i0 i); [|rewrite finmap_get_empty in H0; discriminate].
-    rewrite singleton_get in H0.
-    destruct (eq_dec i1 (fresh _)); inv H0; auto. }
-  { simpl; intros.
-    destruct (eq_dec _ _); [|discriminate].
-    rewrite singleton_get.
-    destruct (eq_dec _ _); inv H0; eauto. }
-  { repeat intro.
-    clear H3; specialize (Hvb i0).
-    destruct (eq_dec i0 i); eauto.
-    rewrite finmap_get_set in H0.
-    destruct (eq_dec i1 (fresh _)); inv H0; eauto. }
-  { simpl; intros.
-    destruct (eq_dec _ _); [|eauto].
-    rewrite finmap_get_set.
-    destruct (eq_dec _ _); eauto. }
-  { apply single_valid; auto. }
+  intros.
+  eapply derives_trans; [apply Own_unit|].
+  apply exp_left; intro g0.
+  apply prop_andp_left; intro Hg0.
+  eapply derives_trans.
+  - apply Own_update_ND with (B := fun b => exists g, b = singleton g (existT _ RA (exist _ _ H), pp)).
+    intros ? c [? J]; exists (singleton (length c) (existT _ RA (exist _ _ H), pp)).
+    split; eauto.
+    rewrite (identity_core Hg0), ghost_core in J; inv J; [|eexists; constructor].
+    rewrite ghost_fmap_singleton; eexists; apply singleton_join_gen.
+    rewrite nth_overflow by auto; constructor.
+  - apply bupd_mono, exp_left; intro g'.
+    apply prop_andp_left; intros [g]; subst.
+    apply exp_right with g.
+    eapply exp_right; eauto.
 Qed.
 
 Lemma singleton_join: forall {A} {J: Join A} a b c k,
@@ -474,53 +328,9 @@ Proof.
   - split.
     + inversion 1; subst.
       inv H3; auto.
-    + repeat constructor; auto.
+    + intro; do 2 constructor; auto.
   - rewrite <- IHk.
     split; [inversion 1 | repeat constructor]; auto.
-Qed.
-
-Lemma single_ghost_join: forall I (I_eq : EqDec I) (RAs: I -> Ghost) RA n
-  (H : RAs (fst n) = RA) a b c, join a b c ->
-  join (single_ghost(H := H) n a) (single_ghost(H := H) n b) (single_ghost(H := H) n c).
-Proof.
-  repeat intro; unfold single_ghost.
-  destruct (eq_dec _ _); [|constructor].
-  apply singleton_join; subst; auto.
-Qed.
-
-Lemma preds_join_refl: forall I a, preds_join I a a a.
-Proof.
-  repeat intro.
-  destruct (a _ _); constructor; auto.
-Qed.
-
-Lemma eq_dec_irr: forall {A} (e1: EqDec A) (e2: EqDec A), e1 = e2.
-Proof.
-  intros; extensionality a b.
-  destruct (e1 a b), (e2 a b); try contradiction; f_equal; apply proof_irr.
-Qed.
-
-Lemma ghost_op: forall {RA: Ghost} g (a1 a2 a3: G) pp,
-  join a1 a2 a3 ->
-  own g a3 pp = own g a1 pp * own g a2 pp.
-Proof.
-  intros; apply pred_ext.
-  - destruct g.
-    repeat (apply exp_left; intro).
-    erewrite Own_op by ((apply single_ghost_join, H) || apply preds_join_refl).
-    apply sepcon_derives; repeat eapply exp_right; eauto.
-  - destruct g.
-    intros ? (w1 & w2 & J & (? & ? & ? & ? & ? & Hg1) & (? & ? & ? & ? & ? & Hg2)).
-    pose proof (ghost_of_join _ _ _ J) as Jg.
-    rewrite Hg1, Hg2 in Jg; inversion Jg.
-    repeat inj_pair_tac.
-    do 3 eexists.
-    erewrite Own_op by ((apply single_ghost_join, H) || apply preds_join_refl).
-    exists w1, w2; repeat split; auto.
-    + replace x4 with x0 by apply eq_dec_irr.
-      eexists; apply Hg1.
-    + replace x2 with x6 by apply proof_irr.
-      eexists; apply Hg2.
 Qed.
 
 Lemma singleton_join_inv: forall {A} {J: Join A} k a b c,
@@ -537,26 +347,35 @@ Lemma ghost_valid_2: forall {RA: Ghost} g a1 a2 pp,
   own g a1 pp * own g a2 pp |-- !!ghost.valid_2 a1 a2.
 Proof.
   intros.
-  destruct g as [? [i]].
-  intros w (? & ? & J%ghost_of_join & (? & ? & ? & ? & ? & Hg1) & (? & ? & e1 & ? & ? & Hg2)).
-  rewrite Hg1, Hg2 in J.
-  inv J; repeat inj_pair_tac.
-  specialize (H3 i); apply finmap_get_join with (i0 := n) in H3.
-  clear H9; specialize (Hvc i n).
-  unfold single_ghost in H3; simpl in H3.
-  destruct (eq_dec i i); [|contradiction].
-  rewrite singleton_get in H3.
-  destruct (eq_dec n n); [|contradiction].
-  destruct (eq_dec i i); [|contradiction].
-  rewrite singleton_get in H3.
-  destruct (eq_dec n n); [|contradiction].
-  destruct (finmap_get (c0 i) n); [|contradiction].
-  subst; simpl in *.
-  eexists; split; eauto.
-  rewrite (UIP_refl _ _ e), (UIP_refl _ _ e1), (UIP_refl _ _ e2) in H3; auto.
+  intros w (? & ? & J%ghost_of_join & (? & ? & Hg1) & (? & ? & Hg2)).
+  rewrite Hg1, Hg2, !ghost_fmap_singleton in J.
+  apply singleton_join_inv in J as ([] & J & ?).
+  inv J; simpl in *.
+  inv H2; repeat inj_pair_tac.
+  eexists; eauto.
 Qed.
 
-Corollary ghost_valid: forall {RA: Ghost} g a pp,
+Lemma ghost_op: forall {RA: Ghost} g (a1 a2 a3: G) pp, join a1 a2 a3 ->
+  own g a3 pp = own g a1 pp * own g a2 pp.
+Proof.
+  intros; apply pred_ext.
+  - apply exp_left; intro.
+    erewrite Own_op; [apply sepcon_derives; eapply exp_right; eauto|].
+    apply singleton_join; constructor; constructor; auto.
+  - eapply derives_trans; [apply andp_right, derives_refl; apply ghost_valid_2|].
+    apply prop_andp_left; intros (? & J & ?).
+    eapply join_eq in H; eauto; subst.
+    unfold own; rewrite exp_sepcon1; apply exp_left; intro.
+    rewrite exp_sepcon2; apply exp_left; intro.
+    erewrite <- Own_op; [eapply exp_right; eauto|].
+    apply singleton_join; constructor; constructor; auto.
+  Unshelve.
+  eapply join_valid; eauto.
+  eapply join_valid; eauto.
+  auto.
+Qed.
+
+Lemma ghost_valid: forall {RA: Ghost} g a pp,
   own g a pp |-- !!ghost.valid a.
 Proof.
   intros.
@@ -567,91 +386,52 @@ Proof.
   apply core_identity in J; subst; auto.
 Qed.
 
-Lemma singleton_join_some: forall {A} {J: Join A} k (a b c: A) m
-  (Hget: finmap_get m k = Some b) (Hjoin: join a b c),
-  join (singleton k a) m (finmap_set m k c).
+Lemma singleton_join_inv_gen: forall k a (b c: ghost),
+  join (singleton k a) b c -> join (Some a) (nth k b None) (nth k c None).
 Proof.
-  unfold finmap_get; induction k; intros.
-  - destruct m; [rewrite nth_nil in Hget; discriminate|].
-    simpl in *; subst; repeat constructor; auto.
-  - destruct m; [discriminate|].
-    repeat constructor; eapply IHk; eauto.
-Qed.
-
-Lemma singleton_join_none: forall {A} {J: Join A} k (a: A) m (Hget: finmap_get m k = None),
-  join (singleton k a) m (finmap_set m k a).
-Proof.
-  unfold finmap_get; induction k; intros.
-  - destruct m; simpl in *; subst; repeat constructor.
-  - destruct m; repeat constructor; eapply IHk; eauto.
+  unfold singleton; induction k; inversion 1; subst; auto; try constructor.
+  - rewrite app_nth2; rewrite repeat_length; auto.
+    rewrite minus_diag; constructor.
+  - apply IHk; auto.
 Qed.
 
 Lemma ghost_update_ND: forall {RA: Ghost} g (a: G) B pp,
   fp_update_ND a B -> own g a pp |-- bupd (EX b : _, !!(B b) && own g b pp).
 Proof.
   intros.
-  eapply derives_trans; [apply andp_right, derives_refl; apply ghost_valid|].
-  apply prop_andp_left; intro Hva.
-  destruct g as [? [i n]].
-  repeat (apply exp_left; intro).
+  apply exp_left; intro Hva.
   eapply derives_trans.
-  - apply Own_update_ND with (Hv := single_valid (i, n) x2 a Hva)
-      (B0 := fun g => exists b (Hv: ghost.valid b), B b /\ g = GHOST _ _ _ _ (single_valid (i, n) x2 b Hv) (single_dom (i, n) x2 b pp)).
+  - apply Own_update_ND with
+      (B := fun b => exists b' Hvb, B b' /\ b = singleton g (existT _ RA (exist _ b' Hvb), pp)).
     intros ?? [? J].
-    inv J; repeat inj_pair_tac.
-    pose proof (H6 i) as J; specialize (Hvc i n).
-    apply finmap_get_join with (i0 := n) in J.
-    unfold single_ghost in J; simpl in J.
-    destruct (eq_dec i i); [|contradiction].
-    rewrite singleton_get, if_true in J by auto.
-    destruct (finmap_get (b0 i) n) eqn: Hb.
-    + destruct (finmap_get (c1 i) n); [|contradiction].
-      rewrite (UIP_refl _ _ e) in J.
-      lapply (H g); [|eexists; eauto].
-      intros (b & ? & g' & J' & Hvg'); simpl in *.
-      pose proof (singleton_join_some _ _ _ _ _ Hb J').
-      pose proof (join_valid _ _ _ J' Hvg') as Hvb'.
-      eexists; split; [exists b, Hvb'; eauto|].
-      eexists; constructor; eauto; simpl.
-      instantiate (1 := fun j => match eq_dec j i with
-        left H => finmap_set (b0 j) n (eq_rect_r (fun j => @G (x1 j)) g' H) | _ => b0 j end).
-      unfold single_ghost; simpl.
-      intro j; destruct (eq_dec j i); [|constructor].
-      subst; auto.
-    + lapply (H (core a)).
-      intros (b & ? & ? & J' & ?).
-      apply join_valid in J'; auto.
-      eexists; split; [exists b, J'; eauto|].
-      eexists; constructor; eauto; simpl.
-      instantiate (1 := fun j => match eq_dec j i with
-        left H => _ | _ => b0 j end).
-      unfold single_ghost; simpl.
-      intro j; destruct (eq_dec j i); [|constructor].
-      apply singleton_join_none; subst; auto.
-      { eexists; split; eauto; apply join_comm, core_unit. }
-  - apply bupd_mono.
-    repeat (apply exp_left; intro); apply prop_andp_left; intros (? & ? & ? & Hg).
-    inv Hg; repeat inj_pair_tac.
-    eapply exp_right, andp_right; [repeat intro; simpl; eauto|].
-    repeat eapply exp_right.
-    replace x6 with (single_dom (i, n) (eq_refl _) x7 pp) by apply proof_irr; auto.
+    rewrite ghost_fmap_singleton in J.
+    pose proof (singleton_join_inv_gen _ _ _ _ J) as Jg.
+    inv Jg.
+    + destruct (H (core a)) as (b & ? & Hv).
+      { eexists; split; [apply join_comm, core_unit | auto]. }
+      assert (ghost.valid b) as Hvb.
+      { destruct Hv as (? & ? & ?); eapply join_valid; eauto. }
+      exists (singleton g (existT _ RA (exist _ _ Hvb), pp)); split; eauto.
+      rewrite ghost_fmap_singleton.
+      eexists; apply singleton_join_gen.
+      rewrite <- H2; constructor.
+    + destruct a2, a3; inv H3; simpl in *.
+      inv H0; inj_pair_tac.
+      destruct (H b0) as (b & ? & Hv).
+      { eexists; eauto. }
+      destruct Hv as (? & ? & ?).
+      assert (ghost.valid b) as Hvb by (eapply join_valid; eauto).
+      exists (singleton g (existT _ RA (exist _ _ Hvb), pp)); split; eauto.
+      rewrite ghost_fmap_singleton.
+      eexists; apply singleton_join_gen.
+      instantiate (1 := (_, _)).
+      rewrite <- H1; constructor; constructor; [constructor|]; eauto.
+  - apply bupd_mono, exp_left; intro.
+    apply prop_andp_left; intros (b & ? & ? & ?); subst.
+    apply exp_right with b, prop_andp_right; auto.
+    eapply exp_right; auto.
   Unshelve.
-  { intros j m ??; specialize (Hvb j m).
-    destruct (eq_dec j i); auto.
-    rewrite finmap_get_set in H2.
-    destruct (eq_dec m n); inv H2; auto. }
-  { intros j m ??; specialize (H7 j m); unfold single_pred in H7; simpl in *.
-    destruct (eq_dec _ _); [|eapply domb; inv H7; rewrite H2 in *; eauto].
-    rewrite finmap_get_set; destruct (eq_dec _ _); eauto.
-    eapply domb; inv H7; rewrite H2 in *; eauto. }
-  { intros j m ??; specialize (Hvb j m).
-    destruct (eq_dec j i); auto.
-    rewrite finmap_get_set in H2.
-    destruct (eq_dec m n); inv H2; auto. }
-  { intros j m ??; specialize (H7 j m); unfold single_pred in H7; simpl in *.
-    destruct (eq_dec _ _); [|eapply domb; inv H7; rewrite H2 in *; eauto].
-    rewrite finmap_get_set; destruct (eq_dec _ _); eauto.
-    eapply domb; inv H7; rewrite H2 in *; eauto. }
+  auto.
 Qed.
 
 Lemma ghost_update: forall {RA: Ghost} g (a b: G) pp,
