veric/rmaps.v
@@ -49,7 +49,8 @@ Inductive TypeTree: Type :=
   | DependentType: nat -> TypeTree
   | ProdType: TypeTree -> TypeTree -> TypeTree
   | ArrowType: TypeTree -> TypeTree -> TypeTree
-  | PiType: forall (I : Type), (I -> TypeTree) -> TypeTree.
+  | PiType: forall (I : Type), (I -> TypeTree) -> TypeTree
+  | ListType: TypeTree -> TypeTree.
 
 Definition dependent_type_functor_rec (ts: list Type): TypeTree -> functor :=
   fix dtfr (T: TypeTree): functor :=
@@ -60,6 +61,7 @@ Definition dependent_type_functor_rec (ts: list Type): TypeTree -> functor :=
   | ProdType T1 T2 => fpair (dtfr T1) (dtfr T2)
   | ArrowType T1 T2 => ffunc (dtfr T1) (dtfr T2)
   | PiType _ f => fpi (fun i => dtfr (f i))
+  | ListType T => flist (dtfr T)
   end.
 Opaque dependent_type_functor_rec.
 
@@ -72,189 +74,30 @@ Definition dependent_type_function_rec (ts: list Type) (mpred': Type): TypeTree 
   | ProdType T1 T2 => (dtfr T1 * dtfr T2)%type
   | ArrowType T1 T2 => dtfr T1 -> dtfr T2
   | PiType A f => forall a, dtfr (f a)
+  | ListType T => list (dtfr T)
   end.
 
 Definition fpreds: functor :=
   fsig (fun T: TypeTree =>
     fpi (fun ts: list Type => dependent_type_functor_rec ts T)).
 
-Instance preds_join (PRED : Type) (I: Type) : Join (I -> nat -> option (fpreds PRED)) :=
-  Join_fun _ _ (Join_fun _ _ (Join_lower (Join_equiv (fpreds PRED)))).
-
-Section Finmap.
-
-(* There are a million ways to define a finite map. I want one that:
-   can be used generically (so cannot defined as a module),
-   provides a function that returns a fresh index,
-   and has extensional equivalence as its equality. *)
-Definition finmap A := list (option A).
-
-Import ListNotations.
-Definition finmap_set {A} (m : finmap A) k v : finmap A :=
-  firstn k m ++ repeat None (k - length m) ++ Some v :: skipn (S k) m.
-
-Definition finmap_get {A} (m : finmap A) k := nth k m None.
-
-Lemma nth_firstn: forall {A} m (l : list A) n d, m < length (firstn n l) ->
-  nth m (firstn n l) d = nth m l d.
+Lemma realize_eq: forall {A} (a b: A) P, (exists H: a = b, P H) -> {H: a = b & P H}.
 Proof.
-  induction m; destruct l, n; auto; simpl; intros; try omega.
-  apply IHm; omega.
+  intros ???? []; subst; exists eq_refl; auto.
 Qed.
 
-Lemma nth_repeat: forall {A} m n (x : A), nth m (repeat x n) x = x.
-Proof.
-  induction m; destruct n; simpl; intros; auto.
-Qed.
-
-Lemma nth_nil: forall {A} n (d : A), nth n [] d = d.
-Proof.
-  destruct n; auto.
-Qed.
-
-Lemma nth_skipn: forall {A} n m (l : list A) d, nth m (skipn n l) d = nth (m + n) l d.
-Proof.
-  induction n; simpl; intros.
-  { rewrite Nat.add_0_r; auto. }
-  destruct l.
-  { rewrite !nth_nil; auto. }
-  rewrite IHn, Nat.add_succ_r; auto.
-Qed.
-
-Opaque skipn.
-
-Lemma finmap_get_empty: forall {A} i, finmap_get (@nil (option A)) i = None.
-Proof.
-  intros; apply nth_nil.
-Qed.
-
-Lemma finmap_get_set: forall {A} (m : finmap A) j k v,
-  finmap_get (finmap_set m k v) j = if eq_dec j k then Some v else finmap_get m j.
-Proof.
-  intros; unfold finmap_get, finmap_set.
-  destruct (eq_dec j k).
-  - subst.
-    rewrite 2app_nth2; rewrite ?firstn_length, ?repeat_length.
-    replace (_ - _) with O; auto.
-    all: destruct (Min.min_spec k (length m)) as [[? ->] | [? ->]]; auto; omega.
-  - destruct (lt_dec j (length (firstn k m))).
-    { rewrite app_nth1, nth_firstn; auto. }
-    rewrite app_nth2 by omega.
-    rewrite firstn_length in *.
-    destruct (lt_dec k (length m)).
-    + rewrite Min.min_l in * by omega.
-      replace (k - length m) with O by omega.
-      destruct (j - k) eqn: Hminus; [omega | simpl].
-      rewrite nth_skipn.
-      f_equal; omega.
-    + rewrite Min.min_r in * by omega.
-      rewrite (nth_overflow m) by omega.
-      destruct (lt_dec (j - length m) (k - length m)).
-      { rewrite app_nth1, nth_repeat; auto.
-        rewrite repeat_length; auto. }
-      rewrite app_nth2; rewrite repeat_length; [|omega].
-      destruct (j - length m - (k - length m)) eqn: Hminus; [omega | simpl].
-      rewrite nth_skipn, nth_overflow; auto; omega.
-Qed.
-
-Definition fresh {A} (m : finmap A) := length m.
-Lemma fresh_spec: forall {A} (m : finmap A), finmap_get m (fresh m) = None.
-Proof.
-  unfold fresh, finmap_get; intros; rewrite nth_overflow; auto.
-Qed.
-
-
-Context {A} {J: Join A}.
-
-Inductive finmap_join: Join (finmap A) :=
-| finmap_join_nil_l m: finmap_join [] m m
-| finmap_join_nil_r m: finmap_join m [] m
-| finmap_join_cons a1 a2 m1 m2 a3 m3: join a1 a2 a3 -> finmap_join m1 m2 m3 ->
-    finmap_join (a1 :: m1) (a2 :: m2) (a3 :: m3).
-Hint Constructors finmap_join.
-
-Lemma finmap_join_inv: forall m1 m2 m3, finmap_join m1 m2 m3 ->
-  match m1, m2 with
-  | [], _ => m3 = m2
-  | _, [] => m3 = m1
-  | a1 :: m1, a2 :: m2 => match m3 with [] => False
-                          | a3 :: m3 => join a1 a2 a3 /\ finmap_join m1 m2 m3 end
-  end.
-Proof.
-  induction 1; simpl; auto.
-  destruct m; simpl; auto.
-Qed.
-
-Lemma finmap_get_join: forall m1 m2 m3, finmap_join m1 m2 m3 -> forall i,
-  match finmap_get m1 i, finmap_get m2 i, finmap_get m3 i with
-  | Some a1, Some a2, Some a3 => join a1 a2 a3
-  | None, x, y | x, None, y => y = x
+Lemma lower_join_inv : forall {A} {J: Join A} a b c, lower_join J a b c <->
+  match a, b, c with
+  | Some a, Some b, Some c => join a b c
+  | Some a, None, Some c | None, Some a, Some c => a = c
+  | None, None, None => True
   | _, _, _ => False
   end.
 Proof.
-  unfold finmap_get; induction 1; intros; rewrite ?nth_nil; auto.
-  { destruct (nth i m None); auto. }
-  destruct i; simpl.
-  - inv H; auto.
-    destruct a3; auto.
-  - apply IHfinmap_join.
+  split.
+  - inversion 1; subst; auto; destruct c; auto.
+  - destruct a, b, c; intros; subst; try contradiction; try constructor; auto.
 Qed.
-
-(* Note that maps are not a Disj_alg, since a map containing only cores joins with itself
-   but isn't a universal unit. *)
-Global Instance Perm_finmap {P: Perm_alg A} : @Perm_alg _ finmap_join.
-Proof.
-  constructor.
-  - intros until 1; revert z'; induction H; inversion 1; subst; auto.
-    f_equal; auto.
-    eapply join_eq; eauto.
-  - unfold join; simpl.
-    induction a; intros ???? HJ1 HJ2; apply finmap_join_inv in HJ1; subst; eauto.
-    destruct b; subst; eauto.
-    destruct d; [contradiction|].
-    destruct HJ1 as [Ha1 HJ1].
-    apply finmap_join_inv in HJ2; simpl in HJ2.
-    destruct c; subst; eauto.
-    destruct e; [contradiction|].
-    destruct HJ2 as [Ha2 HJ2].
-    destruct (join_assoc Ha1 Ha2) as (f & ? & ?).
-    destruct (IHa _ _ _ _ HJ1 HJ2) as (f' & ? & ?).
-    exists (f :: f'); auto.
-  - induction 1; constructor; auto.
-  - intros until 1; revert b'; induction H; inversion 1; subst; auto.
-    f_equal; eauto.
-    eapply join_positivity; eauto.
-Qed.
-
-Global Instance Sep_finmap {S: Sep_alg A} : @Sep_alg _ finmap_join.
-Proof.
-  exists (fun _ => nil); auto.
-  constructor.
-Qed.
-
-End Finmap.
-
-Instance finmap_RA {RA: Ghost} : Ghost :=
-  { valid m := forall i a, finmap_get m i = Some a -> valid a; Join_G := finmap_join }.
-Proof.
-  intros.
-  specialize (H0 i).
-  apply finmap_get_join with (i0 := i) in H.
-  rewrite H1 in H.
-  destruct (finmap_get b i); eauto.
-  destruct (finmap_get c i); [|contradiction].
-  eapply join_valid; eauto.
-Defined.
-
-Existing Instance finmap_join.
-
-Instance Global_Ghost {I} {RAs: I -> Ghost}: Ghost :=
-  { G := forall i, finmap (@G (RAs i)); valid m := forall i, @valid finmap_RA (m i) }.
-Proof.
-  intros.
-  specialize (H i).
-  eapply join_valid; eauto.
-Defined.
 
 Module Type STRAT_MODEL.
   Declare Module AV : ADR_VAL.
@@ -312,56 +155,35 @@ Module Type STRAT_MODEL.
       | PURE' _ _ => None (* PUREs cannot be split in any interesting way, which is what valid is about. *)
     end.
 
-  Inductive ghost (PRED : Type) : Type :=
-    GHOST' I (RAs: I -> Ghost) (g: @G Global_Ghost) (pds: I -> nat -> option (fpreds PRED))
-      (Hv: ghost.valid g)
-      (dom: forall i n pp, pds i n = Some pp -> exists a, finmap_get (g i) n = Some a).
+  Definition ghost (PRED : Type) : Type :=
+    list (option ({g: Ghost & {a: @G g | ghost.valid a}} * fpreds PRED)%type).
 
-  Program Definition ghost_fmap (A B:Type) (f:A->B) (g:B->A)(x:ghost A) : ghost B :=
-    match x with
-      | GHOST' _ RAs a pds _ _ =>
-        GHOST' _ _ RAs a (fmap (ffunc (fconst _) (ffunc (fconst _) (foption fpreds))) f g pds) _ _
-    end.
-  Next Obligation.
-  Proof.
-    simpl in H.
-    destruct (pds i n) eqn: Hi; inv H; eauto.
-  Defined.
+  Definition ghost_fmap (A B:Type) (f:A->B) (g:B->A)(x:ghost A) : ghost B :=
+    fmap (flist (foption (fpair (fconst _) fpreds))) f g x.
 
   Axiom ff_ghost : functorFacts ghost ghost_fmap.
   Definition f_ghost : functor := Functor ff_ghost.
 
-  (* Will this give us the higher-order ghost state we want? *)
-  Inductive ghost_join (PRED : Type) : Join (f_ghost PRED) :=
-    | ghost_join_I : forall A (RAs : A -> Ghost) a b c pdsa pdsb pdsc Hva Hvb Hvc doma domb domc,
-        join a b c -> join pdsa pdsb pdsc ->
-        ghost_join PRED (GHOST' PRED _ RAs a pdsa Hva doma) (GHOST' PRED _ RAs b pdsb Hvb domb)
-                        (GHOST' PRED _ RAs c pdsc Hvc domc).
+  Instance preds_join PRED : Join _ := Join_equiv (fpreds PRED).
 
-  Lemma ghost_ext: forall PRED I RAs g g' pds pds' Hv Hv' dom dom',
-    g = g' -> pds = pds' -> GHOST' PRED I RAs g pds Hv dom = GHOST' PRED I RAs g' pds' Hv' dom'.
-  Proof.
-    intros; subst.
-    f_equal; apply proof_irr.
-  Qed.
+  Inductive ghost_elem_join : Join {g: Ghost & {a: @G g | ghost.valid a}} :=
+  | elem_join_I g a b c va vb vc: join a b c ->
+    ghost_elem_join (existT _ g (exist _ a va)) (existT _ g (exist _ b vb))
+                    (existT _ g (exist _ c vc)).
+  Existing Instance ghost_elem_join.
+
+  Inductive ghost_join PRED : Join (ghost PRED) :=
+  | ghost_join_nil_l m: ghost_join PRED nil m m
+  | ghost_join_nil_r m: ghost_join PRED m nil m
+  | ghost_join_cons a1 a2 m1 m2 a3 m3: join a1 a2 a3 -> ghost_join PRED m1 m2 m3 ->
+      ghost_join PRED (a1 :: m1) (a2 :: m2) (a3 :: m3).
+  Existing Instance ghost_join.
 
   Axiom pa_gj : forall PRED, @Perm_alg _ (ghost_join PRED).
 
-  Lemma core_dom: forall {PRED I} {RAs: I -> Ghost} (pds : I -> nat -> option (fpreds PRED))
-    (g: @G Global_Ghost) i n pp, core pds i n = Some pp -> exists a, finmap_get (g i) n = Some a.
-  Proof.
-    discriminate.
-  Qed.
-
   Instance sa_gj : forall PRED, @Sep_alg _ (ghost_join PRED).
   Proof.
-    intros.
-    exists (fun x => match x with GHOST' _ RA g pds Hv _ =>
-                         GHOST' PRED _ RA (core g) (core pds) (core_valid _ Hv) (core_dom _ _) end).
-    - destruct t; constructor; apply core_unit.
-    - intros; inv H.
-      apply ghost_ext; auto.
-      eapply join_core; eauto.
+    intros; exists (fun _ => nil); auto; constructor.
   Defined.
   Axiom paf_ghost : @pafunctor f_ghost ghost_join.
 
@@ -553,215 +375,187 @@ Module StratModel (AV' : ADR_VAL) : STRAT_MODEL with Module AV:=AV'.
       | PURE' _ _ => None (* PUREs cannot be split in any interesting way, which is what valid is about. *)
     end.
 
-  Inductive ghost (PRED : Type) : Type :=
-    GHOST' I (RAs: I -> Ghost) (g: @G Global_Ghost) (pds: I -> nat -> option (fpreds PRED))
-      (Hv: ghost.valid g)
-      (dom: forall i n pp, pds i n = Some pp -> exists a, finmap_get (g i) n = Some a).
+  Definition ghost (PRED : Type) : Type :=
+    list (option ({g: Ghost & {a: @G g | ghost.valid a}} * fpreds PRED)%type).
 
-  Program Definition ghost_fmap (A B:Type) (f:A->B) (g:B->A)(x:ghost A) : ghost B :=
-    match x with
-      | GHOST' _ RAs a pds _ _ =>
-        GHOST' _ _ RAs a (fmap (ffunc (fconst _) (ffunc (fconst _) (foption fpreds))) f g pds) _ _
-    end.
-  Next Obligation.
-  Proof.
-    simpl in H.
-    destruct (pds i n) eqn: Hi; inv H; eauto.
-  Defined.
-
-  Lemma ghost_ext: forall PRED I RAs g g' pds pds' Hv Hv' dom dom',
-    g = g' -> pds = pds' -> GHOST' PRED I RAs g pds Hv dom = GHOST' PRED I RAs g' pds' Hv' dom'.
-  Proof.
-    intros; subst.
-    f_equal; apply proof_irr.
-  Qed.
+  Definition ghost_fmap (A B:Type) (f:A->B) (g:B->A)(x:ghost A) : ghost B :=
+    fmap (flist (foption (fpair (fconst _) fpreds))) f g x.
 
   Lemma ff_ghost : functorFacts ghost ghost_fmap.
   Proof.
-    constructor; intros; extensionality x; icase x; unfold ghost_fmap.
-    - apply ghost_ext; auto.
-      rewrite fmap_id; auto.
-    - apply ghost_ext; auto.
-      rewrite <- fmap_comp; auto.
+    constructor; intros; extensionality x; unfold ghost_fmap.
+    - rewrite fmap_id; auto.
+    - rewrite <- fmap_comp; auto.
   Qed.
 
   Definition f_ghost : functor := Functor ff_ghost.
 
-  (* Will this give us the higher-order ghost state we want? *)
-  Inductive ghost_join (PRED : Type) : f_ghost PRED -> f_ghost PRED -> f_ghost PRED -> Prop :=
-    | ghost_join_I : forall A (RAs : A -> Ghost) a b c pdsa pdsb pdsc Hva Hvb Hvc doma domb domc,
-        join a b c -> join pdsa pdsb pdsc ->
-        ghost_join PRED (GHOST' PRED _ RAs a pdsa Hva doma) (GHOST' PRED _ RAs b pdsb Hvb domb)
-                        (GHOST' PRED _ RAs c pdsc Hvc domc).
-  Lemma ghost_join_inv : forall PRED A RAs a b c pdsa pdsb pdsc Hva Hvb Hvc doma domb domc,
-    ghost_join PRED (GHOST' PRED A RAs a pdsa Hva doma) (GHOST' PRED A RAs b pdsb Hvb domb)
-      (GHOST' PRED A RAs c pdsc Hvc domc) ->
-      join a b c /\ join pdsa pdsb pdsc.
+  Instance preds_join PRED : Join _ := Join_equiv (fpreds PRED).
+
+  Inductive ghost_elem_join : Join {g: Ghost & {a: @G g | ghost.valid a}} :=
+  | elem_join_I g a b c va vb vc: join a b c ->
+    ghost_elem_join (existT _ g (exist _ a va)) (existT _ g (exist _ b vb))
+                    (existT _ g (exist _ c vc)).
+  Existing Instance ghost_elem_join.
+
+  Inductive ghost_join PRED : Join (ghost PRED) :=
+  | ghost_join_nil_l m: ghost_join PRED nil m m
+  | ghost_join_nil_r m: ghost_join PRED m nil m
+  | ghost_join_cons a1 a2 m1 m2 a3 m3: join a1 a2 a3 -> ghost_join PRED m1 m2 m3 ->
+      ghost_join PRED (a1 :: m1) (a2 :: m2) (a3 :: m3).
+  Hint Constructors ghost_join.
+  Existing Instance ghost_join.
+
+  Lemma elem_join_inv: forall a1 a2 a3, ghost_elem_join a1 a2 a3 ->
+  match a1, a2, a3 with
+  | existT g1 (exist x1 _), existT g2 (exist x2 _), existT g3 (exist x3 _) =>
+      exists H: g2 = g1, exists H': g3 = g1, join x1 (eq_rect _ _ x2 _ H) (eq_rect _ _ x3 _ H')
+  end.
   Proof.
-    inversion 1.
-    repeat (match goal with H : existT _ _ _ = existT _ _ _ |- _ => apply inj_pair2 in H end;
-      subst); auto.
+    inversion 1; subst.
+    exists eq_refl, eq_refl; auto.
   Qed.
 
-  Instance Join_ghost (PRED: Type) : Join (ghost PRED) := ghost_join PRED.
+  Lemma ghost_join_inv: forall PRED m1 m2 m3, ghost_join PRED m1 m2 m3 ->
+  match m1, m2 with
+  | nil, _ => m3 = m2
+  | _, nil => m3 = m1
+  | a1 :: m1, a2 :: m2 => match m3 with nil => False
+                          | a3 :: m3 => join a1 a2 a3 /\ ghost_join PRED m1 m2 m3 end
+  end.
+  Proof.
+    induction 1; simpl; auto.
+    destruct m; simpl; auto.
+  Qed.
+
+  Instance pa_gej : @Perm_alg _ ghost_elem_join.
+  Proof.
+    constructor.
+    - inversion 1; inversion 1; subst.
+      inv H.
+      repeat (match goal with H : existT _ _ _ = existT _ _ _ |- _ => apply inj_pair2 in H end;
+          subst).
+      f_equal; eapply exist_ext, join_eq; eauto.
+    - intros ????? J1%elem_join_inv J2%elem_join_inv.
+      destruct a as (ga & a & ?), b as (gb & b & ?), c as (gc & c & ?), d as (gd & d & ?),
+        e as (ge & e & ?).
+      repeat (apply realize_eq in J1; destruct J1 as [? J1]).
+      repeat (apply realize_eq in J2; destruct J2 as [? J2]); subst.
+      destruct (join_assoc J1 J2) as (f & ? & J).
+      exists (existT _ ga (exist _ f (join_valid _ _ _ (join_comm J) v3))).
+      split; constructor; auto.
+    - inversion 1; constructor; auto.
+    - inversion 1; subst; inversion 1; subst; auto.
+      inv H.
+      repeat (match goal with H : existT _ _ _ = existT _ _ _ |- _ => apply inj_pair2 in H end;
+          subst).
+      f_equal; eapply exist_ext, join_positivity; eauto.
+  Qed.
 
   Instance pa_gj : forall PRED, @Perm_alg _ (ghost_join PRED).
   Proof.
-    constructor; intros.
-    - inv H; inv H0.
-      repeat (match goal with H : existT _ _ _ = existT _ _ _ |- _ => apply inj_pair2 in H end;
-          subst).
-      apply ghost_ext; eapply join_eq; eauto.
-    - destruct a as [I RA a pdsa], b as [I1 RA1 b pdsb], d as [I2 RA2 d pdsd].
-      assert (I1 = I /\ I2 = I) as [] by (inv H; auto); subst.
-      assert (RA1 = RA /\ RA2 = RA) as []; subst.
-      { inv H.
-        repeat (match goal with H : existT _ _ _ = existT _ _ _ |- _ => apply inj_pair2 in H end;
-          subst); auto. }
-      apply ghost_join_inv in H as [J1 J1'].
-      destruct c as [I1 RA1 c pdsc], e as [I2 RA2 e pdse].
-      assert (I1 = I /\ I2 = I) as [] by (inv H0; auto); subst.
-      assert (RA1 = RA /\ RA2 = RA) as []; subst.
-      { inv H0.
-        repeat (match goal with H : existT _ _ _ = existT _ _ _ |- _ => apply inj_pair2 in H end;
-          subst); auto. }
-      apply ghost_join_inv in H0 as [J2 J2'].
-      destruct (join_assoc J1 J2) as (f & ? & ?).
-      destruct (join_assoc J1' J2') as (pdsf & ? & ?).
-      assert (ghost.valid f) as Hvf by (eapply join_valid; eauto).
-      assert (forall i n pp, pdsf i n = Some pp -> exists a, finmap_get (f i) n = Some a)
-        as domf.
-      { intros.
-        specialize (H i); specialize (H1 i n).
-        apply finmap_get_join with (i0 := n) in H.
-        destruct (finmap_get (f i) n); eauto.
-        inv H1.
-        + rewrite H3 in H7; destruct (dom2 _ _ _ H7) as [? Hget].
-          rewrite Hget in H.
-          destruct (finmap_get (b i) n); inv H.
-        + rewrite H3 in H7; destruct (dom0 _ _ _ H7) as [? Hget].
-          rewrite Hget in H.
-          destruct (finmap_get (c i) n); inv H.
-        + symmetry in H4; destruct (dom0 _ _ _ H4) as [? Hget].
-          rewrite Hget in H.
-          destruct (finmap_get (c i) n); inv H. }
-      exists (GHOST' PRED _ RA f pdsf Hvf domf); split; constructor; auto.
-    - inv H; constructor; apply join_comm; auto.
-    - inv H; inv H0.
-      repeat (match goal with H : existT _ _ _ = existT _ _ _ |- _ => apply inj_pair2 in H end;
-        subst); auto.
-      apply ghost_ext; eapply join_positivity; eauto.
-  Qed.
-
-  Lemma core_dom: forall {PRED I} {RAs: I -> Ghost} (pds : I -> nat -> option (fpreds PRED))
-    (g: @G Global_Ghost) i n pp, core pds i n = Some pp -> exists a, finmap_get (g i) n = Some a.
-  Proof.
-    discriminate.
+    constructor.
+    - intros until 1; revert z'; induction H; inversion 1; subst; auto.
+      f_equal; auto.
+      eapply join_eq; eauto.
+    - induction a; intros ???? J1 J2; apply ghost_join_inv in J1; subst.
+      { exists e; split; auto; constructor. }
+      destruct b; subst; [eexists; split; eauto; constructor|].
+      destruct d; [contradiction|].
+      destruct J1 as [Jc1 J1].
+      apply ghost_join_inv in J2.
+      destruct c; subst; [eexists; split; eauto; constructor; auto|].
+      destruct e; [contradiction|].
+      destruct J2 as [Jc2 J2].
+      destruct (join_assoc Jc1 Jc2) as (f & ? & ?).
+      destruct (IHa _ _ _ _ J1 J2) as (f' & ? & ?).
+      exists (f :: f'); split; constructor; auto.
+    - induction 1; constructor; auto.
+    - intros until 1; revert b'; induction H; inversion 1; subst; auto.
+      f_equal; eauto.
+      eapply join_positivity; eauto.
   Qed.
 
   Instance sa_gj : forall PRED, @Sep_alg _ (ghost_join PRED).
   Proof.
-    intros.
-    exists (fun x => match x with GHOST' _ RA g pds Hv _ =>
-                         GHOST' PRED _ RA (core g) (core pds) (core_valid _ Hv) (core_dom _ _) end).
-    - destruct t; constructor; apply core_unit.
-    - intros; inv H.
-      apply ghost_ext; auto.
-      eapply join_core; eauto.
+    intros; exists (fun _ => nil); auto; constructor.
   Defined.
+
+  Opaque fpreds.
 
   Definition paf_ghost : @pafunctor f_ghost ghost_join.
   Proof.
     constructor; repeat intro.
-    - inv H; constructor; auto.
-      intros i n; specialize (H1 i n); inv H1; simpl.
-      + rewrite <- H2, H; constructor.
-      + rewrite <- H3, H4; constructor.
-      + inv H4.
-        rewrite <- H, <- H2, <- H3; repeat constructor.
-    - destruct x' as [I RA x pds], y as [I1 RA1 y pds1], z as [I2 RA2 z pds2].
-      assert (I1 = I /\ I2 = I) as [] by (inv H; auto); subst.
-      assert (RA1 = RA /\ RA2 = RA) as []; subst.
-      { inv H.
-        repeat match goal with H : existT _ _ _ = existT _ _ _ |- _ => apply inj_pair2 in H end;
-          subst; auto. }
-      apply ghost_join_inv in H as [J J'].
-      eexists (GHOST' A _ RA x (fun i n => match pds i n with Some _ => pds2 i n | _ => None end) Hv _),
-        (GHOST' A _ RA y (fun i n => match pds1 i n with Some _ => pds2 i n | _ => None end) Hv0 _);
-        repeat split; auto.
-      + intros i n; specialize (J' i n); inv J'.
-        * destruct (pds1 i n), (pds2 i n); inv H; constructor.
-        * destruct (pds1 i n); inv H1.
-          destruct (pds i n), (pds2 i n); inv H2; constructor.
-        * destruct (pds1 i n); inv H0.
-          destruct (pds2 i n); inv H1; constructor; auto.
-      + apply ghost_ext; auto.
-        extensionality i n; specialize (J' i n); inv J'; auto; simpl.
-        * rewrite <- H0; auto.
-        * rewrite H2.
-          destruct (pds2 i n); auto.
-        * rewrite <- H.
-          destruct (pds1 i n); inv H0.
-          destruct (pds2 i n); inv H1.
-          inv H2; auto.
-      + apply ghost_ext; auto; simpl.
-        extensionality i n; specialize (J' i n); inv J'; auto.
-        * destruct (pds1 i n), (pds2 i n); inv H; auto.
-        * destruct (pds1 i n); inv H1; auto.
-        * destruct (pds1 i n); inv H0.
-          destruct (pds2 i n); inv H1.
-          inv H2; auto.
-    - destruct x as [I RA x pds], y as [I1 RA1 y pds1], z' as [I2 RA2 z pds2].
-      assert (I1 = I /\ I2 = I) as [] by (inv H; auto); subst.
-      assert (RA1 = RA /\ RA2 = RA) as []; subst.
-      { inv H.
-        repeat match goal with H : existT _ _ _ = existT _ _ _ |- _ => apply inj_pair2 in H end;
-          subst; auto. }
-      apply ghost_join_inv in H as [J J'].
-      eexists (GHOST' A _ RA y (fun i n => match pds i n, pds1 i n with Some x, Some _ => Some x
-          | _, _ => pds1 i n end) Hv0 _),
-        (GHOST' A _ RA z (fun i n => match pds i n with Some x => Some x | None => pds1 i n end) Hv1 _);
-        repeat split; auto.
-      + intros i n; specialize (J' i n); inv J'.
-        * destruct (pds i n); inv H0; constructor.
-        * destruct (pds1 i n); inv H1.
-          destruct (pds i n); constructor.
-        * destruct (pds i n); inv H.
-          destruct (pds1 i n); inv H0; constructor; auto.
-      + apply ghost_ext; auto; simpl.
-        extensionality i n; specialize (J' i n); inv J'; auto.
-        * destruct (pds i n); inv H0; constructor.
-        * destruct (pds1 i n); inv H1.
-          destruct (pds i n); constructor.
-        * destruct (pds i n); inv H.
-          destruct (pds1 i n); inv H0.
-          inv H2; auto.
-      + apply ghost_ext; auto; simpl.
-        extensionality i n; specialize (J' i n); inv J'; auto.
-        * destruct (pds i n); inv H0; constructor.
-        * destruct (pds1 i n); inv H1.
-          destruct (pds i n); constructor.
-        * destruct (pds i n); inv H.
-          destruct (pds1 i n); inv H0.
-          inv H2; auto.
-    Unshelve.
-    simpl; intros; destruct (pds i n) eqn: Hi; inv H; eauto.
-    simpl; intros; destruct (pds1 i n) eqn: Hi; inv H; eauto.
-    simpl; intros; destruct (pds i n) eqn: Hi, (pds1 i n) eqn: Hi1; inv H; eauto.
-    simpl; intros.
-    specialize (J i); specialize (J' i n); apply finmap_get_join with (i0 := n) in J.
-    destruct (finmap_get (z i) n); eauto.
-    inv J'.
-    destruct (pds i n); inv H1.
-    destruct (dom0 _ _ _ H) as [? Hget]; rewrite Hget in J.
-    destruct (finmap_get (x i) n); inv J.
-    destruct (pds1 i n); inv H2.
-    destruct (pds i n) eqn: Hi; inv H.
-    destruct (dom _ _ _ Hi) as [? Hget]; rewrite Hget in J.
-    destruct (finmap_get (y i) n); inv J.
-    destruct (pds i n) eqn: Hi; inv H0.
-    destruct (dom _ _ _ Hi) as [? Hget]; rewrite Hget in J.
-    destruct (finmap_get (y i) n); inv J.
+    - induction H; constructor; auto.
+      inv H; constructor; auto.
+      inv H1; constructor; auto.
+      inv H2; constructor; auto; simpl; congruence.
+    - revert dependent z; revert y; induction x'; intros; apply ghost_join_inv in H.
+      { exists nil, z; split; auto; constructor. }
+      destruct y; simpl in *.
+      { exists z, nil; split; auto; constructor. }
+      destruct z; [contradiction | simpl in *].
+      destruct H as [J1 J2].
+      destruct (IHx' _ _ J2) as (x & y' & ? & ? & ?); subst.
+      apply lower_join_inv in J1.
+      destruct a as [[[? []]]|].
+      + destruct o as [[[? []]]|].
+        * destruct o0 as [[[? []]]|]; [|contradiction].
+          destruct J1 as [J1%elem_join_inv J1']; simpl in *.
+          repeat (apply realize_eq in J1 as [? J1]); subst; simpl in *.
+          exists (Some (existT _ x0 (exist _ _ v), _f1) :: x),
+            (Some (existT _ x0 (exist _ _ v0), _f1) :: y').
+          split; [repeat constructor; auto|].
+          unfold ghost_fmap in *; simpl in *.
+          inv J1'.
+          rewrite <- H1, <- H2; auto.
+        * destruct o0 as [[[? []]]|]; [|contradiction].
+          inv J1.
+          match goal with H : existT _ _ _ = existT _ _ _ |- _ => apply inj_pair2 in H end;
+            subst.
+          exists (Some (existT _ x2 (exist _ _ v0), _f0) :: x), (None :: y').
+          split; [repeat constructor; auto|].
+          unfold ghost_fmap in *; simpl in *.
+          rewrite <- H1; split; f_equal; f_equal; f_equal; f_equal.
+          apply exist_ext; auto.
+      + exists (None :: x), (o0 :: y').
+        split; [repeat constructor; auto|].
+        split; auto.
+        unfold ghost_fmap in *; simpl in *.
+        rewrite <- H1; f_equal.
+        destruct o, o0; inv J1; auto.
+    - revert dependent z'; revert y; induction x; intros; apply ghost_join_inv in H; simpl in H.
+      { exists y, y; split; auto; constructor. }
+      destruct y; simpl in *.
+      { exists nil, (a :: x); split; auto; constructor. }
+      destruct z'; [contradiction | simpl in *].
+      destruct H as [J1 J2].
+      destruct (IHx _ _ J2) as (y' & z & ? & ? & ?); subst.
+      apply lower_join_inv in J1.
+      destruct a as [[[? []]]|].
+      + destruct o as [[[? []]]|].
+        * destruct o0 as [[[? []]]|]; [|contradiction].
+          destruct J1 as [J1%elem_join_inv J1']; simpl in *.
+          repeat (apply realize_eq in J1 as [? J1]); subst; simpl in *.
+          exists (Some (existT _ x0 (exist _ _ v0), _f) :: y'),
+            (Some (existT _ x0 (exist _ _ v1), _f) :: z).
+          split; [repeat constructor; auto|].
+          unfold ghost_fmap in *; simpl in *.
+          inv J1'.
+          rewrite <- H0, <- H1; auto.
+        * destruct o0 as [[[? []]]|]; [|contradiction].
+          inv J1.
+          match goal with H : existT _ _ _ = existT _ _ _ |- _ => apply inj_pair2 in H end;
+            subst.
+          exists (None :: y'), (Some (existT _ x2 (exist _ _ v), _f) :: z).
+          split; [repeat constructor; auto|].
+          unfold ghost_fmap in *; simpl in *.
+          rewrite <- H0; split; f_equal; f_equal; f_equal; f_equal.
+          apply exist_ext; auto.
+      + exists (o :: y'), (o :: z).
+        split; [repeat constructor; auto|].
+        unfold ghost_fmap in *; simpl in *; rewrite <- H0; split; f_equal.
+        destruct o, o0; auto; contradiction.
   Qed.
 
   Definition valid' A (w: (address -> res A) * ghost A) : Prop :=
@@ -795,7 +589,7 @@ Module StratModel (AV' : ADR_VAL) : STRAT_MODEL with Module AV:=AV'.
   Definition f_pre_rmap : functor :=
     fsubset (fpair (ffunc (fconst address) f_res) f_ghost) _ valid'_res_map.
 
-  Notation Join_obj A := (Join_prod _ (Join_fun address (res A) (res_join A)) _ (Join_ghost A)).
+  Notation Join_obj A := (Join_prod _ (Join_fun address (res A) (res_join A)) _ (ghost_join A)).
 
   Instance Join_pre_rmap (A: Type) : Join (pre_rmap A) :=
     Join_prop _ (Join_obj A) (valid' A).
@@ -912,9 +706,6 @@ Module Type RMAPS.
   Axiom preds_fmap_comp : forall f1 f2 g1 g2,
     preds_fmap g1 g2 oo preds_fmap f1 f2 = preds_fmap (g1 oo f1) (f2 oo g2).
 
-  Instance preds_join (I: Type) : Join (I -> nat -> option preds) :=
-    Join_fun _ _ (Join_fun _ _ (Join_lower (Join_equiv preds))).
-
   Definition resource_fmap (f g:pred rmap -> pred rmap) (x:resource) : resource :=
     match x with
     | NO sh nsh => NO sh nsh
@@ -925,52 +716,29 @@ Module Type RMAPS.
   Axiom resource_fmap_comp : forall f1 f2 g1 g2,
     resource_fmap g1 g2 oo resource_fmap f1 f2 = resource_fmap (g1 oo f1) (f2 oo g2).
 
-  Inductive ghost : Type := GHOST I (RA : I -> Ghost) (g : @G Global_Ghost) (pds : I -> nat -> option preds)
-    (Hv : ghost.valid g)
-    (dom : forall i n pp, pds i n = Some pp -> exists a, finmap_get (g i) n = Some a).
+  Definition ghost : Type := list (option ({g: Ghost & {a: @G g | ghost.valid a}} * preds)%type).
 
-  Lemma ghost_ext: forall I RAs g g' pds pds' Hv Hv' dom dom',
-    g = g' -> pds = pds' -> GHOST I RAs g pds Hv dom = GHOST I RAs g' pds' Hv' dom'.
-  Proof.
-    intros; subst.
-    f_equal; apply proof_irr.
-  Qed.
+  Instance preds_join : Join _ := Join_equiv preds.
 
-  (* Will this give us the higher-order ghost state we want? *)
-  Inductive ghost_join : ghost -> ghost -> ghost -> Prop :=
-    | ghost_join_I : forall A (RA : A -> Ghost) a b c pdsa pdsb pdsc Hva Hvb Hvc doma domb domc, join a b c ->
-        join pdsa pdsb pdsc ->
-        ghost_join (GHOST _ RA a pdsa Hva doma) (GHOST _ RA b pdsb Hvb domb) (GHOST _ RA c pdsc Hvc domc).
-  Lemma ghost_join_inv : forall A RAs a b c pdsa pdsb pdsc Hva Hvb Hvc doma domb domc,
-    ghost_join (GHOST A RAs a pdsa Hva doma) (GHOST A RAs b pdsb Hvb domb) (GHOST A RAs c pdsc Hvc domc) ->
-    join a b c /\ join pdsa pdsb pdsc.
-  Proof.
-    inversion 1.
-    repeat (match goal with H : existT _ _ _ = existT _ _ _ |- _ => apply inj_pair2 in H end;
-      subst); auto.
-  Qed.
+  Inductive ghost_elem_join : Join {g: Ghost & {a: @G g | ghost.valid a}} :=
+  | elem_join_I g a b c va vb vc: join a b c ->
+    ghost_elem_join (existT _ g (exist _ a va)) (existT _ g (exist _ b vb))
+                    (existT _ g (exist _ c vc)).
+  Existing Instance ghost_elem_join.
 
-  Lemma core_dom: forall {I} {RAs: I -> Ghost} (pds : I -> nat -> option preds)
-    (g: @G Global_Ghost) i n pp, core pds i n = Some pp -> exists a, finmap_get (g i) n = Some a.
-  Proof.
-    discriminate.
-  Qed.
+  Inductive ghost_join : Join ghost :=
+  | ghost_join_nil_l m: ghost_join nil m m
+  | ghost_join_nil_r m: ghost_join m nil m
+  | ghost_join_cons a1 a2 m1 m2 a3 m3: join a1 a2 a3 -> ghost_join m1 m2 m3 ->
+      ghost_join (a1 :: m1) (a2 :: m2) (a3 :: m3).
+  Existing Instance ghost_join.
 
-  Instance Join_ghost : Join ghost := ghost_join.
   Axiom Perm_ghost: Perm_alg ghost. Existing Instance Perm_ghost.
   Axiom Sep_ghost: Sep_alg ghost. Existing Instance Sep_ghost.
-  Axiom ghost_core: forall A (RA : A -> Ghost) a pds Hv dom,
-    core (GHOST _ RA a pds Hv dom) = GHOST _ RA (core a) (core pds) (core_valid _ Hv) (core_dom _ _).
+  Axiom ghost_core: forall (g: ghost), core g = nil.
 
-  Program Definition ghost_fmap (f g:pred rmap -> pred rmap)(x:ghost) : ghost :=
-    match x with
-      | GHOST _ RA a pds _ _ => GHOST _ RA a (fun i n => option_map (preds_fmap f g) (pds i n)) _ _
-    end.
-  Next Obligation.
-  Proof.
-    simpl in H.
-    destruct (pds i n) eqn: Hi; inv H; eauto.
-  Defined.
+  Definition ghost_fmap (f g:pred rmap -> pred rmap)(x:ghost) : ghost :=
+    map (option_map (fun '(a, b) => (a, preds_fmap f g b))) x.
 
   Axiom ghost_fmap_id : ghost_fmap (id _) (id _) = id ghost.
   Axiom ghost_fmap_comp : forall f1 f2 g1 g2,
@@ -1109,9 +877,7 @@ Module Rmaps (AV':ADR_VAL): RMAPS with Module AV:=AV'.
     extensionality r; destruct r; simpl; auto; destruct p; auto.
   Qed.
 
-  Inductive ghost : Type := GHOST I (RAs : I -> Ghost) (g : @G Global_Ghost) (pds : I -> nat -> option preds)
-    (Hv : ghost.valid g)
-    (dom : forall i n pp, pds i n = Some pp -> exists a, finmap_get (g i) n = Some a).
+  Definition ghost : Type := list (option ({g: Ghost & {a: @G g | ghost.valid a}} * preds)%type).
 
   Definition pred2p (p: preds) : fpreds (pred rmap) :=
     match p with SomeP A P => existT _ A P end.
@@ -1119,41 +885,24 @@ Module Rmaps (AV':ADR_VAL): RMAPS with Module AV:=AV'.
   Definition p2pred (p: fpreds (pred rmap)) : preds :=
     match p with existT A P => SomeP A P end.
 
-  Program Definition ghost2g (r: ghost): SM.ghost (pred rmap) :=
-    match r with
-      | GHOST _ RA g pds _ _ => GHOST' (pred rmap) _ RA g (fun i n => option_map pred2p (pds i n)) _ _
-    end.
-  Next Obligation.
-  Proof.
-    destruct (pds i n) eqn: Hi; inv H; eauto.
-  Defined.
+  Definition ghost2g (r: ghost): SM.ghost (pred rmap) :=
+    map (option_map (fun '(a, b) => (a, pred2p b))) r.
 
-  Program Definition g2ghost (r: SM.ghost (pred rmap)) : ghost :=
-    match r with
-      | GHOST' _ RA g pds _ _ => GHOST _ RA g (fun i n => option_map p2pred (pds i n)) _ _
-    end.
-  Next Obligation.
-  Proof.
-    destruct (pds i n) eqn: Hi; inv H; eauto.
-  Defined.
-
-  Lemma ghost_ext: forall I RAs g g' pds pds' Hv Hv' dom dom',
-    g = g' -> pds = pds' -> GHOST I RAs g pds Hv dom = GHOST I RAs g' pds' Hv' dom'.
-  Proof.
-    intros; subst.
-    f_equal; apply proof_irr.
-  Qed.
+  Definition g2ghost (r: SM.ghost (pred rmap)) : ghost :=
+    map (option_map (fun '(a, b) => (a, p2pred b))) r.
 
   Lemma g2ghost2g: forall x, ghost2g (g2ghost x) = x.
   Proof.
-    destruct x; apply SM.ghost_ext; auto.
-    extensionality i n; destruct (pds i n) as [[]|]; auto.
+    induction x; auto; simpl.
+    rewrite IHx; destruct a as [[]|]; auto; simpl.
+    destruct _f; auto.
   Qed.
 
   Lemma ghost2g2ghost: forall x, g2ghost (ghost2g x) = x.
   Proof.
-    destruct x; apply ghost_ext; auto.
-    extensionality i n; destruct (pds i n) as [[]|]; auto.
+    induction x; auto; simpl.
+    rewrite IHx; destruct a as [[]|]; auto; simpl.
+    destruct p; auto.
   Qed.
 
   Definition valid (m: (address -> resource) * ghost) : Prop :=
@@ -1250,93 +999,101 @@ Module Rmaps (AV':ADR_VAL): RMAPS with Module AV:=AV'.
   intros. inversion H; auto.
   Defined.
 
-  Instance preds_join (I: Type) : Join (I -> nat -> option preds) :=
-    Join_fun _ _ (Join_fun _ _ (Join_lower (Join_equiv preds))).
-
   (* Will this give us the higher-order ghost state we want? *)
-  Inductive ghost_join : ghost -> ghost -> ghost -> Prop :=
-    | ghost_join_I : forall A (RA : A -> Ghost) a b c pdsa pdsb pdsc Hva Hvb Hvc doma domb domc, join a b c ->
-        join pdsa pdsb pdsc ->
-        ghost_join (GHOST _ RA a pdsa Hva doma) (GHOST _ RA b pdsb Hvb domb) (GHOST _ RA c pdsc Hvc domc).
+  Instance preds_join : Join _ := Join_equiv preds.
 
-  Lemma ghost_join_inv : forall A RAs a b c pdsa pdsb pdsc Hva Hvb Hvc doma domb domc,
-    ghost_join (GHOST A RAs a pdsa Hva doma) (GHOST A RAs b pdsb Hvb domb) (GHOST A RAs c pdsc Hvc domc) ->
-    join a b c /\ join pdsa pdsb pdsc.
+  Inductive ghost_elem_join : Join {g: Ghost & {a: @G g | ghost.valid a}} :=
+  | elem_join_I g a b c va vb vc: join a b c ->
+    ghost_elem_join (existT _ g (exist _ a va)) (existT _ g (exist _ b vb))
+                    (existT _ g (exist _ c vc)).
+  Existing Instance ghost_elem_join.
+
+  Inductive ghost_join : Join ghost :=
+  | ghost_join_nil_l m: ghost_join nil m m
+  | ghost_join_nil_r m: ghost_join m nil m
+  | ghost_join_cons a1 a2 m1 m2 a3 m3: join a1 a2 a3 -> ghost_join m1 m2 m3 ->
+      ghost_join (a1 :: m1) (a2 :: m2) (a3 :: m3).
+  Existing Instance ghost_join.
+
+  Lemma elem_join_inv: forall a1 a2 a3, ghost_elem_join a1 a2 a3 ->
+  match a1, a2, a3 with
+  | existT g1 (exist x1 _), existT g2 (exist x2 _), existT g3 (exist x3 _) =>
+      exists H: g2 = g1, exists H': g3 = g1, join x1 (eq_rect _ _ x2 _ H) (eq_rect _ _ x3 _ H')
+  end.
   Proof.
-    inversion 1.
-    repeat (match goal with H : existT _ _ _ = existT _ _ _ |- _ => apply inj_pair2 in H end;
-      subst); auto.
+    inversion 1; subst.
+    exists eq_refl, eq_refl; auto.
   Qed.
 
-  Instance Join_ghost : Join ghost := ghost_join.
+  Lemma ghost_join_inv: forall m1 m2 m3, ghost_join m1 m2 m3 ->
+  match m1, m2 with
+  | nil, _ => m3 = m2
+  | _, nil => m3 = m1
+  | a1 :: m1, a2 :: m2 => match m3 with nil => False
+                          | a3 :: m3 => join a1 a2 a3 /\ ghost_join m1 m2 m3 end
+  end.
+  Proof.
+    induction 1; simpl; auto.
+    destruct m; simpl; auto.
+  Qed.
+
+  Instance pa_gej : @Perm_alg _ ghost_elem_join.
+  Proof.
+    constructor.
+    - inversion 1; inversion 1; subst.
+      inv H.
+      repeat (match goal with H : existT _ _ _ = existT _ _ _ |- _ => apply inj_pair2 in H end;
+          subst).
+      f_equal; eapply exist_ext, join_eq; eauto.
+    - intros ????? J1%elem_join_inv J2%elem_join_inv.
+      destruct a as (ga & a & ?), b as (gb & b & ?), c as (gc & c & ?), d as (gd & d & ?),
+        e as (ge & e & ?).
+      repeat (apply realize_eq in J1; destruct J1 as [? J1]).
+      repeat (apply realize_eq in J2; destruct J2 as [? J2]); subst.
+      destruct (join_assoc J1 J2) as (f & ? & J).
+      exists (existT _ ga (exist _ f (join_valid _ _ _ (join_comm J) v3))).
+      split; constructor; auto.
+    - inversion 1; constructor; auto.
+    - inversion 1; subst; inversion 1; subst; auto.
+      inv H.
+      repeat (match goal with H : existT _ _ _ = existT _ _ _ |- _ => apply inj_pair2 in H end;
+          subst).
+      f_equal; eapply exist_ext, join_positivity; eauto.
+  Qed.
 
   Instance Perm_ghost : Perm_alg ghost.
   Proof.
-    constructor; intros.
-    - inv H; inv H0.
-      repeat (match goal with H : existT _ _ _ = existT _ _ _ |- _ => apply inj_pair2 in H end;
-          subst).
-      apply ghost_ext; eapply join_eq; eauto.
-    - destruct a as [I RA a pdsa], b as [I1 RA1 b pdsb], d as [I2 RA2 d pdsd].
-      assert (I1 = I /\ I2 = I) as [] by (inv H; auto); subst.
-      assert (RA1 = RA /\ RA2 = RA) as []; subst.
-      { inv H.
-        repeat (match goal with H : existT _ _ _ = existT _ _ _ |- _ => apply inj_pair2 in H end;
-          subst); auto. }
-      apply ghost_join_inv in H as [J1 J1'].
-      destruct c as [I1 RA1 c pdsc], e as [I2 RA2 e pdse].
-      assert (I1 = I /\ I2 = I) as [] by (inv H0; auto); subst.
-      assert (RA1 = RA /\ RA2 = RA) as []; subst.
-      { inv H0.
-        repeat (match goal with H : existT _ _ _ = existT _ _ _ |- _ => apply inj_pair2 in H end;
-          subst); auto. }
-      apply ghost_join_inv in H0 as [J2 J2'].
-      destruct (join_assoc J1 J2) as (f & ? & ?).
-      destruct (join_assoc J1' J2') as (pdsf & ? & ?).
-      assert (ghost.valid f) as Hvf by (eapply join_valid; eauto).
-      assert (forall i n pp, pdsf i n = Some pp -> exists a, finmap_get (f i) n = Some a)
-        as domf.
-      { intros.
-        specialize (H i); specialize (H1 i n).
-        apply finmap_get_join with (i0 := n) in H.
-        destruct (finmap_get (f i) n); eauto.
-        inv H1.
-        + rewrite H3 in H7; destruct (dom2 _ _ _ H7) as [? Hget].
-          rewrite Hget in H.
-          destruct (finmap_get (b i) n); inv H.
-        + rewrite H3 in H7; destruct (dom0 _ _ _ H7) as [? Hget].
-          rewrite Hget in H.
-          destruct (finmap_get (c i) n); inv H.
-        + symmetry in H4; destruct (dom0 _ _ _ H4) as [? Hget].
-          rewrite Hget in H.
-          destruct (finmap_get (c i) n); inv H. }
-      exists (GHOST _ RA f pdsf Hvf domf); split; constructor; auto.
-    - inv H; constructor; apply join_comm; auto.
-    - inv H; inv H0.
-      repeat (match goal with H : existT _ _ _ = existT _ _ _ |- _ => apply inj_pair2 in H end;
-        subst); auto.
-      apply ghost_ext; eapply join_positivity; eauto.
-  Qed.
-
-  Lemma core_dom: forall {I} {RAs: I -> Ghost} (pds : I -> nat -> option preds)
-    (g: @G Global_Ghost) i n pp, core pds i n = Some pp -> exists a, finmap_get (g i) n = Some a.
-  Proof.
-    discriminate.
+    constructor.
+    - intros until 1; revert z'; induction H; inversion 1; subst; auto.
+      f_equal; auto.
+      eapply join_eq; eauto.
+    - induction a; intros ???? J1 J2; apply ghost_join_inv in J1; subst.
+      { exists e; split; auto; constructor. }
+      destruct b; subst; [eexists; split; eauto; constructor|].
+      destruct d; [contradiction|].
+      destruct J1 as [Jc1 J1].
+      apply ghost_join_inv in J2.
+      destruct c; subst; [eexists; split; eauto; constructor; auto|].
+      destruct e; [contradiction|].
+      destruct J2 as [Jc2 J2].
+      destruct (join_assoc Jc1 Jc2) as (f & ? & ?).
+      destruct (IHa _ _ _ _ J1 J2) as (f' & ? & ?).
+      exists (f :: f'); split; constructor; auto.
+    - induction 1; constructor; auto.
+    - intros until 1; revert b'; induction H; inversion 1; subst; auto.
+      f_equal; eauto.
+      eapply join_positivity; eauto.
   Qed.
 
   Instance Sep_ghost : Sep_alg ghost.
   Proof.
-    intros.
-    exists (fun x => match x with GHOST _ RA g pds Hv _ => GHOST _ RA (core g) (core pds) (core_valid _ Hv) (core_dom _ _) end).
-    - destruct t; constructor; apply core_unit.
-    - intros; inv H.
-      apply ghost_ext; auto.
-      eapply join_core; eauto.
+    intros; exists (fun _ => nil); auto; constructor.
   Defined.
 
-  Lemma ghost_core : forall A (RA : A -> Ghost) a pds Hv dom,
-    core (GHOST _ RA a pds Hv dom) = GHOST _ RA (core a) (core pds) (core_valid _ Hv) (core_dom _ _).
-  Proof. auto. Qed.
+  Lemma ghost_core : forall (g: ghost), core g = nil.
+  Proof.
+    auto.
+  Qed.
 
   Lemma same_valid : forall f1 f2, (forall x, f1 x = f2 x) -> AV.valid f1 -> AV.valid f2.
   Proof.
@@ -1410,15 +1167,8 @@ Module Rmaps (AV':ADR_VAL): RMAPS with Module AV:=AV'.
     | PURE k p => PURE k (preds_fmap f g p)
     end.
 
-  Program Definition ghost_fmap (f g:pred rmap -> pred rmap)(x:ghost) : ghost :=
-    match x with
-      | GHOST _ RA a pds _ _ => GHOST _ RA a (fun i n => option_map (preds_fmap f g) (pds i n)) _ _
-    end.
-  Next Obligation.
-  Proof.
-    simpl in H.
-    destruct (pds i n) eqn: Hi; inv H; eauto.
-  Defined.
+  Definition ghost_fmap (f g:pred rmap -> pred rmap)(x:ghost) : ghost :=
+    map (option_map (fun '(a, b) => (a, preds_fmap f g b))) x.
 
   Lemma valid_res_map : forall f g m, valid m -> valid (resource_fmap f g oo fst m, ghost_fmap f g (snd m)).
   Proof.
@@ -1442,10 +1192,9 @@ Module Rmaps (AV':ADR_VAL): RMAPS with Module AV:=AV'.
 
   Lemma ghost_fmap_id : ghost_fmap (id (pred rmap)) (id (pred rmap)) = id ghost.
   Proof.
-    extensionality x; destruct x; apply ghost_ext; auto.
-    rewrite preds_fmap_id; unfold id; f_equal.
-    extensionality i n.
-    destruct (pds i n); auto.
+    extensionality x; induction x; auto; simpl.
+    rewrite IHx; destruct a as [[]|]; auto; simpl.
+    rewrite preds_fmap_id; auto.
   Qed.
 
   Lemma resource_fmap_comp : forall f1 f2 g1 g2,
@@ -1461,9 +1210,8 @@ Module Rmaps (AV':ADR_VAL): RMAPS with Module AV:=AV'.
   Lemma ghost_fmap_comp : forall f1 f2 g1 g2,
     ghost_fmap g1 g2 oo ghost_fmap f1 f2 = ghost_fmap (g1 oo f1) (f2 oo g2).
   Proof.
-    intros; extensionality x; destruct x; apply ghost_ext; auto.
-    extensionality i n.
-    destruct (pds i n); auto; simpl.
+    intros; extensionality x; induction x; auto; simpl.
+    rewrite <- IHx; destruct a as [[]|]; auto; simpl.
     rewrite <- preds_fmap_comp; auto.
   Qed.
 
@@ -1642,11 +1390,10 @@ Module Rmaps (AV':ADR_VAL): RMAPS with Module AV:=AV'.
     destruct p; simpl.
     rewrite approx_K_approx; auto.
     (* ghost *)
-    destruct g; simpl.
-    apply ghost_ext; auto.
-    extensionality i m.
-    destruct (pds i m) as [[]|]; auto; simpl.
-    rewrite approx_K_approx; auto.
+    clear v; induction g; auto; simpl.
+    setoid_rewrite IHg; destruct a as [[]|]; auto; simpl.
+    repeat f_equal.
+    rewrite approx_K_approx; destruct p; auto.
   Qed.
 
   Instance Join_nat_rmap': Join (nat * rmap') := Join_prod _ (Join_equiv nat) _ _.
@@ -1672,6 +1419,14 @@ Proof.
   apply equal_f with k in H0. rewrite H0; intuition.
 Qed.
 *)
+  Lemma g2ghost_inv: forall g1 g2, g2ghost g1 = g2ghost g2 -> g1 = g2.
+  Proof.
+    induction g1; destruct g2; inversion 1; auto.
+    f_equal; auto.
+    destruct a as [[]|], o as [[]|]; inv H1; auto.
+    destruct _f, _f0; inv H4; auto.
+  Qed.
+
   Lemma join_unsquash : forall phi1 phi2 phi3,
     join phi1 phi2 phi3 <->
     join (unsquash phi1) (unsquash phi2) (unsquash phi3).
@@ -1702,10 +1457,11 @@ Qed.
     constructor; auto.
 
     destruct f, f0, f1; simpl in *.
-    destruct x, x0, x1; simpl in *; inv H2; simpl.
-    constructor; auto.
-    intros i m; specialize (H4 i m); inv H4; constructor.
-    inv H7; auto.
+    destruct x, x0, x1; simpl in *.
+    clear - H2; induction H2; constructor; auto.
+    inv H; constructor; auto.
+    destruct a0, a4, a5; inv H0; simpl in *.
+    inv H; inv H1; constructor; constructor; auto.
 
     destruct H; simpl in *; split; simpl; auto.
     destruct f as [f ?].
@@ -1734,17 +1490,25 @@ Qed.
       constructor; auto.
     + simpl in *.
       destruct f, f0, f1; simpl in *.
-      destruct g, g0, g1; simpl in *.
-      inv H2.
-      repeat (match goal with H : existT _ _ _ = existT _ _ _ |- _ => apply inj_pair2 in H end;
-        subst); constructor; auto.
-      intros i m; specialize (H16 i m); inv H16; destruct (pds i m), (pds0 i m), (pds1 i m);
-        try discriminate; try constructor.
-      * destruct s, s0; inv H6; constructor.
-      * destruct s, s0; inv H6; constructor.
-      * inv H2; inv H3; inv H4.
-        destruct s, s0, s1; inv H6.
-        inv H3; inv H2; auto.
+      clear - H2.
+      remember (g2ghost g) as a; remember (g2ghost g0) as b; remember (g2ghost g1) as c.
+      revert dependent g1; revert dependent g0; revert dependent g; induction H2; intros; subst.
+      * apply g2ghost_inv in Heqc; subst; destruct g; [constructor | discriminate].
+      * apply g2ghost_inv in Heqc; subst; destruct g0; [constructor | discriminate].
+      * destruct g, g0, g1; inv Heqa; inv Heqb; inv Heqc.
+        constructor; [|apply IHghost_join; auto].
+        destruct o as [[]|], o0 as [[]|], o1 as [[]|]; inv H; try constructor.
+        -- destruct _f, _f0, _f1; inv H4; simpl in *.
+           inv H; inv H0.
+           inv H; inv H3.
+           repeat (match goal with H : existT _ _ _ = existT _ _ _ |- _ => apply inj_pair2 in H end;
+             subst); constructor; constructor; auto.
+        -- destruct _f, _f0; inv H4.
+           repeat (match goal with H : existT _ _ _ = existT _ _ _ |- _ => apply inj_pair2 in H end;
+             subst); constructor; auto.
+        -- destruct _f, _f0; inv H4.
+           repeat (match goal with H : existT _ _ _ = existT _ _ _ |- _ => apply inj_pair2 in H end;
+             subst); constructor; auto.
   Qed.
 
   Lemma ghost_of_core : forall phi, ghost_of (core phi) = core (ghost_of phi).
@@ -1754,10 +1518,7 @@ Qed.
     destruct (K.unsquash phi); simpl.
     rewrite K.unsquash_squash.
     destruct (pre_rmap_core _ _f).
-    setoid_rewrite H; simpl.
-    destruct _f as [[]]; simpl.
-    destruct _f0; simpl.
-    apply ghost_ext; auto.
+    setoid_rewrite H; auto.
   Qed.
 
   Definition rmap_age1 (k:rmap) : option rmap :=
